dafny/StreamProcessorTests.dfy
@@ -1,0 +1,82 @@
+include "Utilities.dfy"
+include "StreamProcessor.dfy"
+
+module StreamProcessorTestsModule {
+  import Utils = UtilitiesModule
+  import SP = StreamProcessorModule
+
+  method {:test} Test_SP_ModeSwitch(sp: SP.StreamProcessor, column: Utils.arrayOfLength12<bool>)
+    modifies sp
+  {
+    var res1 := sp.HandleInput(SP.TEXT, column, false);
+    assert sp.stream_mode == SP.TEXT;
+    var res2 := sp.HandleInput(SP.BINARY, column, false);
+    assert sp.stream_mode == SP.BINARY;
+  }
+
+  method {:test} Test_SP_Handle_CardEnded_TEXT(sp: SP.StreamProcessor, column: Utils.arrayOfLength12<bool>) returns (res: SP.HandleInputResult)
+    modifies sp
+    ensures sp.stream_mode == SP.TEXT
+    ensures res.output_ready
+    ensures res.output_char == '\n'
+    ensures res.output_bytes == []
+  {
+    res := sp.HandleInput(SP.TEXT, column, true);
+  }
+
+  method {:test} Test_SP_Handle_CardEnded_BINARY(sp: SP.StreamProcessor, column: Utils.arrayOfLength12<bool>) returns (res: SP.HandleInputResult)
+    modifies sp
+    ensures sp.stream_mode == SP.BINARY
+    ensures res.output_ready
+    ensures res.output_char == '?'
+    ensures res.output_bytes == [0x0A as bv8]
+  {
+    res := sp.HandleInput(SP.BINARY, column, true);
+  }
+
+  method Test_SP_Handle_Column_TEXT(sp: SP.StreamProcessor, column: Utils.arrayOfLength12<bool>) returns (res: SP.HandleInputResult)
+    modifies sp
+    ensures sp.stream_mode == SP.TEXT
+    ensures res.output_ready
+    ensures res.output_char == sp.GetEBCDICChar(sp.ColumnToInteger(column))
+    ensures res.output_bytes == []
+  {
+    res := sp.HandleInput(SP.TEXT, column, false);
+  }
+
+  method {:test} Test_SP_Handle_Column_BINARY(sp: SP.StreamProcessor, column: Utils.arrayOfLength12<bool>) returns (res: SP.HandleInputResult)
+    modifies sp
+    ensures sp.stream_mode == SP.BINARY
+    ensures res.output_ready
+    ensures res.output_char == '?'
+    ensures res.output_bytes == sp.ColumnToBytes(column)
+  {
+    res := sp.HandleInput(SP.BINARY, column, false);
+  }
+
+  method {:test} Test_SP_EBCDIC_char_whitespace_TEXT(sp: SP.StreamProcessor) returns (res: SP.HandleInputResult)
+    modifies sp
+    requires sp.stream_mode == SP.TEXT
+  {
+    // 0x40 = 0d64 -> 0b 0000 0100 0000 (padded to 12 bits).
+    var column := Utils.SeqToArr12_bool([false, false, false, false, false, true, false, false, false, false, false, false]);
+    res := sp.HandleInput(SP.TEXT, column, false);
+    assert sp.stream_mode == SP.TEXT;
+    assert res.output_ready;
+    assert res.output_char == sp.GetEBCDICChar(sp.ColumnToInteger(column));
+    assert res.output_bytes == [];
+  }
+
+  method {:test} Test_SP_EBCDIC_char_whitespace_BINARY(sp: SP.StreamProcessor) returns (res: SP.HandleInputResult)
+    modifies sp
+    requires sp.stream_mode == SP.BINARY
+  {
+    // 0x40 = 0d64 -> 0b 0000 0100 0000 (padded to 12 bits).
+    var column := Utils.SeqToArr12_bool([false, false, false, false, false, true, false, false, false, false, false, false]);
+    res := sp.HandleInput(SP.BINARY, column, false);
+    assert sp.stream_mode == SP.BINARY;
+    assert res.output_ready;
+    assert res.output_char == '?';
+    assert res.output_bytes == sp.ColumnToBytes(column);
+  }
+}
